crypto_examples/mulntt_ct/ntt_index.dfy
@@ -20,4 +20,23 @@ module ntt_index {
         pow2_basics(len);
         seq(len.full/2, n requires 0 <= n < len.full/2 => a[n * 2 + 1])
     }
+
+    function method {:opaque} merge_even_odd_indexed_items<T>(a: seq<T>, b: seq<T>, len: pow2_t): (r: seq<T>)
+        requires |a| == |b| == len.full;
+        ensures |r| == pow2_double(len).full;
+        ensures even_indexed_items(r, pow2_double(len)) == a;
+        ensures odd_indexed_items(r, pow2_double(len)) == b;
+    {
+        pow2_basics(len);
+        var new_len := pow2_double(len);
+        var r := seq(new_len.full, n requires 0 <= n < new_len.full => 
+            if n % 2 == 0 then a[n/2] else b[n/2]);
+        assert even_indexed_items(r, new_len) == a by {
+            reveal even_indexed_items();
+        }
+        assert odd_indexed_items(r, new_len) == b by {
+            reveal odd_indexed_items();
+        }
+        r
+    }
 }
